Make Montgomery example use row-wise flatten (involves adding Nat.max, List.tl, and List.hd to the pipeline)

src/Experiments/SimplyTypedArithmetic.v
@@ -987,9 +987,9 @@ Module Rows.
     Proof. cbv [eval]; autorewrite with push_map push_sum; reflexivity. Qed.
     Hint Rewrite eval_app : push_eval.
 
-    Definition extract_row (inp : cols) : cols * list Z := (map (@tl _) inp, map (hd 0) inp).
+    Definition extract_row (inp : cols) : cols * list Z := (map (fun c => tl c) inp, map (fun c => hd 0 c) inp).
 
-    Definition max_column_size (x:cols) := fold_right Nat.max 0%nat (map (@length Z) x).
+    Definition max_column_size (x:cols) := fold_right (fun a b => Nat.max a b) 0%nat (map (fun c => length c) x).
 
     Definition from_columns' n start_state : cols * rows :=
       fold_right (fun _ (state : cols * rows) =>
@@ -1158,10 +1158,11 @@ Module Rows.
     Local Notation fw := (fun i => weight (S i) / weight i) (only parsing).
 
     Definition sum_rows' start_state (row1 row2 : list Z) : list Z * Z :=
-      fold_left (fun (state : list Z * Z) next =>
+      fold_right (fun next (state : list Z * Z) =>
                     let i := length (fst state) in (* length of output accumulator tells us the index of [next] *)
-                    let sum_carry := Z.add_with_get_carry_full (fw i) (snd state) (fst next) (snd next) in
-                    (fst state ++ [fst sum_carry], snd sum_carry)) (combine row1 row2) start_state.
+                    dlet_nd next := next in (* makes the output correctly bind variables *)
+                    dlet_nd sum_carry := Z.add_with_get_carry_full (fw i) (snd state) (fst next) (snd next) in
+                    (fst state ++ [fst sum_carry], snd sum_carry)) start_state (rev (combine row1 row2)).
     Definition sum_rows := sum_rows' (nil,0).
 
     Definition flatten' (start_state : list Z * Z) (inp : rows) : list Z * Z :=
@@ -1189,8 +1190,8 @@ Module Rows.
         /\ snd (sum_rows' start_state row1 row2) 
            = (eval nm (row1' ++ row1) + eval nm (row2' ++ row2)) / (weight nm).
     Proof.
-      cbv [sum_rows'].
-      induction row1 as [|x1 row1]; intros;
+      cbv [sum_rows' Let_In].
+      induction row1 as [|x1 row1]; intros; rewrite fold_left_rev_right in *;
         destruct row2 as [|x2 row2]; distr_length; [ subst n | ];
           repeat match goal with
                  | _ => progress autorewrite with natsimplify list
@@ -1201,6 +1202,7 @@ Module Rows.
       specialize (IHrow1 (pred n) (S m)).
       replace (pred n + S m)%nat with (n + m)%nat in IHrow1 by omega.
       rewrite (app_cons_app_app _ row1'), (app_cons_app_app _ row2').
+      rewrite <-fold_left_rev_right.
       apply IHrow1; clear IHrow1; autorewrite with cancel_pair distr_length; try omega;
         repeat match goal with
                | H : ?LHS = _ |- _ =>
@@ -1266,8 +1268,8 @@ Module Rows.
           nth_default 0 (fst (sum_rows' start_state row1 row2)) i
           = ((eval nm (row1' ++ row1) + eval nm (row2' ++ row2)) mod (weight (S i))) / (weight i).
     Proof.
-      cbv [sum_rows'].
-      induction row1 as [|x1 row1]; intros;
+      cbv [sum_rows' Let_In].
+      induction row1 as [|x1 row1]; intros; rewrite fold_left_rev_right in *;
         destruct row2 as [|x2 row2]; distr_length; [ subst n | ];
           repeat match goal with
                  | _ => progress cbn [fold_left]
@@ -1279,6 +1281,7 @@ Module Rows.
       specialize (IHrow1 (pred n) (S m)).
       replace (pred n + S m)%nat with (n + m)%nat in IHrow1 by omega.
       rewrite (app_cons_app_app _ row1'), (app_cons_app_app _ row2').
+      rewrite <-fold_left_rev_right.
       apply IHrow1; clear IHrow1; autorewrite with cancel_pair distr_length; try omega;
         repeat match goal with
                | _ => progress intros
@@ -1510,10 +1513,10 @@ Module MulConverted.
       let p3_a := Associational.mul p1_a p2_a in
       (* important not to use Positional.carry here; we don't want to accumulate yet *)
       let p3'_a := fold_right (fun i acc => Associational.carry (w' i) (w' (S i) / w' i) acc) p3_a (rev idxs) in
-      fst (Columns.flatten w (Columns.from_associational w n3 p3'_a)).
+      fst (Rows.flatten w (Rows.from_associational w n3 p3'_a)).
 
       Hint Rewrite
-           @Columns.eval_from_associational
+           @Rows.eval_from_associational
            @Associational.eval_carry
            @Associational.eval_mul
            @Positional.eval_to_associational
@@ -1531,12 +1534,10 @@ Module MulConverted.
         Positional.eval w n3 (mul_converted n1 n2 m1 m2 n3 idxs p1 p2) = (Positional.eval w n1 p1) * (Positional.eval w n2 p2).
       Proof.
         cbv [mul_converted]; intros.
-        rewrite Columns.flatten_mod by auto using Columns.length_from_associational.
+        rewrite Rows.flatten_mod by eauto using Rows.length_from_associational.
         autorewrite with push_eval. auto using Z.mod_small.
       Qed.
       Hint Rewrite eval_mul_converted : push_eval.
-
-      Hint Rewrite @Columns.length_from_associational : distr_length.
 
       Lemma mul_converted_mod n1 n2 m1 m2 n3 idxs p1 p2  (_:n3<>0%nat) (_:m1<>0%nat) (_:m2<>0%nat):
         length p1 = n1 -> length p2 = n2 ->
@@ -1544,7 +1545,7 @@ Module MulConverted.
         nth_default 0 (mul_converted n1 n2 m1 m2 n3 idxs p1 p2) 0 = (Positional.eval w n1 p1 * Positional.eval w n2 p2) mod (w 1).
       Proof.
         intros; cbv [mul_converted].
-        erewrite Columns.flatten_partitions by (auto; distr_length).
+        rewrite Rows.flatten_partitions with (n:=n3) by (eauto using Rows.length_from_associational; omega).
         autorewrite with distr_length push_eval natsimplify.
         rewrite w_0; autorewrite with zsimplify.
         reflexivity.
@@ -1559,7 +1560,7 @@ Module MulConverted.
         nth_default 0 (mul_converted n1 n2 m1 m2 n3 idxs p1 p2) 1 = (Positional.eval w n1 p1 * Positional.eval w n2 p2) / (w 1).
       Proof.
         intros; subst n3; cbv [mul_converted].
-        erewrite Columns.flatten_partitions by (auto; distr_length).
+        rewrite Rows.flatten_partitions with (n:=2%nat) by (eauto using Rows.length_from_associational; omega).
         autorewrite with distr_length push_eval.
         rewrite Z.mod_small; omega.
       Qed.
@@ -2245,6 +2246,7 @@ Module Compilers.
           | primitive {t:type.primitive} (v : interp t) : ident () t
           | Let_In {tx tC} : ident (tx * (tx -> tC)) tC
           | Nat_succ : ident nat nat
+          | Nat_max : ident (nat * nat) nat
           | Nat_mul : ident (nat * nat) nat
           | Nat_add : ident (nat * nat) nat
           | nil {t} : ident () (list t)
@@ -2265,6 +2267,8 @@ Module Compilers.
           | List_partition {A} : ident ((A -> bool) * list A) (list A * list A)
           | List_app {A} : ident (list A * list A) (list A)
           | List_rev {A} : ident (list A) (list A)
+          | List_tl {A} : ident (list A) (list A)
+          | List_hd {A} : ident (A * list A) A
           | List_fold_right {A B} : ident ((B * A -> A) * A * list B) A
           | List_update_nth {T} : ident (nat * (T -> T) * list T) (list T)
           | List_nth_default {T} : ident (T * list T * nat) T
@@ -2313,6 +2317,7 @@ Module Compilers.
                | Nat_succ => Nat.succ
                | Nat_add => curry2 Nat.add
                | Nat_mul => curry2 Nat.mul
+               | Nat_max => curry2 Nat.max
                | nil t => curry0 (@Datatypes.nil (type.interp t))
                | cons t => curry2 (@Datatypes.cons (type.interp t))
                | fst A B => @Datatypes.fst (type.interp A) (type.interp B)
@@ -2331,6 +2336,8 @@ Module Compilers.
                | List_partition A => curry2 (@List.partition (type.interp A))
                | List_app A => curry2 (@List.app (type.interp A))
                | List_rev A => @List.rev (type.interp A)
+               | List_tl A => @List.tl (type.interp A)
+               | List_hd A => curry2 (@List.hd (type.interp A))
                | List_fold_right A B => curry3_1 (@List.fold_right (type.interp A) (type.interp B))
                | List_update_nth T => curry3 (@update_nth (type.interp T))
                | List_nth_default T => curry3 (@List.nth_default (type.interp T))
@@ -2362,6 +2369,7 @@ Module Compilers.
             | Nat.succ ?x => mkAppIdent Nat_succ x
             | Nat.add ?x ?y => mkAppIdent Nat_add (x, y)
             | Nat.mul ?x ?y => mkAppIdent Nat_mul (x, y)
+            | Nat.max ?x ?y => mkAppIdent Nat_max (x, y)
             | S ?x => mkAppIdent Nat_succ x
             | @Datatypes.nil ?T
               => let rT := type.reify T in
@@ -2451,6 +2459,12 @@ Module Compilers.
             | @List.rev ?A ?ls
               => let rA := type.reify A in
                  mkAppIdent (@ident.List_rev rA) ls
+            | @List.tl ?A ?ls
+              => let rA := type.reify A in
+                 mkAppIdent (@ident.List_tl rA) ls
+            | @List.hd ?A ?x ?ls
+              => let rA := type.reify A in
+                 mkAppIdent (@ident.List_hd rA) (x, ls)
             | @List.fold_right ?A ?B (fun b a => ?f) ?a0 ?ls
               => let rA := type.reify A in
                  let rB := type.reify B in
@@ -2505,6 +2519,8 @@ Module Compilers.
             Notation partition := List_partition.
             Notation app := List_app.
             Notation rev := List_rev.
+            Notation tl := List_tl.
+            Notation hd := List_hd.
             Notation fold_right := List_fold_right.
             Notation update_nth := List_update_nth.
             Notation nth_default := List_nth_default.
@@ -2533,6 +2549,7 @@ Module Compilers.
             Notation succ := Nat_succ.
             Notation add := Nat_add.
             Notation mul := Nat_mul.
+            Notation max := Nat_max.
           End Nat.
 
           Module Export Notations.
@@ -2576,6 +2593,7 @@ Module Compilers.
           | Nat_succ : ident nat nat
           | Nat_add : ident (nat * nat) nat
           | Nat_mul : ident (nat * nat) nat
+          | Nat_max : ident (nat * nat) nat
           | nil {t} : ident () (list t)
           | cons {t} : ident (t * list t) (list t)
           | fst {A B} : ident (A * B) A
@@ -2651,6 +2669,7 @@ Module Compilers.
                  | Nat_succ => Nat.succ
                  | Nat_add => curry2 Nat.add
                  | Nat_mul => curry2 Nat.mul
+                 | Nat_max => curry2 Nat.max
                  | nil t => curry0 (@Datatypes.nil (type.interp t))
                  | cons t => curry2 (@Datatypes.cons (type.interp t))
                  | fst A B => @Datatypes.fst (type.interp A) (type.interp B)
@@ -2709,6 +2728,7 @@ Module Compilers.
             | Nat.succ ?x => mkAppIdent Nat_succ x
             | Nat.add ?x ?y => mkAppIdent Nat_add (x, y)
             | Nat.mul ?x ?y => mkAppIdent Nat_mul (x, y)
+            | Nat.max ?x ?y => mkAppIdent Nat_max (x, y)
             | S ?x => mkAppIdent Nat_succ x
             | @Datatypes.nil ?T
               => let rT := type.reify T in
@@ -2832,6 +2852,7 @@ Module Compilers.
             Notation succ := Nat_succ.
             Notation add := Nat_add.
             Notation mul := Nat_mul.
+            Notation max := Nat_max.
           End Nat.
 
           Module Export Notations.
@@ -2897,6 +2918,8 @@ Module Compilers.
                => AppIdent ident.Nat_add
              | for_reification.ident.Nat_mul
                => AppIdent ident.Nat_mul
+             | for_reification.ident.Nat_max
+               => AppIdent ident.Nat_max
              | for_reification.ident.nil t
                => AppIdent ident.nil
              | for_reification.ident.cons t
@@ -3067,6 +3090,28 @@ Module Compilers.
                                      nil
                                      (fun x l' rev_l' => List_app rev_l' [x])
                                      ls) in
+                    let v := app_and_maybe_cancel v in exact v)
+             | for_reification.ident.List_tl A
+               => ltac:(
+                    let v := reify
+                               (@expr var)
+                               (fun ls
+                                => list_rect
+                                     (fun _ => list (type.interp A))
+                                     nil
+                                     (fun _ l' _ => l')
+                                     ls) in
+                    let v := app_and_maybe_cancel v in exact v)
+             | for_reification.ident.List_hd A
+               => ltac:(
+                    let v := reify
+                               (@expr var)
+                               (fun (xls : type.interp A * list (type.interp A))
+                                => list_rect
+                                     (fun _ => type.interp A)
+                                     (fst xls)
+                                     (fun x _ _ => x)
+                                     (snd xls)) in
                     let v := app_and_maybe_cancel v in exact v)
              | for_reification.ident.List_fold_right A B
                => ltac:(
@@ -3692,6 +3737,7 @@ Module Compilers.
                   | ident.Nat_succ as idc
                   | ident.Nat_add as idc
                   | ident.Nat_mul as idc
+                  | ident.Nat_max as idc
                   | ident.pred as idc
                   | ident.Z_shiftr _ as idc
                   | ident.Z_shiftl _ as idc
@@ -3883,6 +3929,7 @@ Module Compilers.
                             @@ (ident.fst @@ (Var xyk)))
                 | ident.Nat_add as idc
                 | ident.Nat_mul as idc
+                | ident.Nat_max as idc
                   => λ (xyk :
                           (* ignore this line; it's to work around lack of fixpoint refolding in type inference *) var (type.nat * type.nat * (type.nat -> R))%ctype) ,
                      (ident.snd @@ (Var xyk))
@@ -4585,6 +4632,7 @@ Module Compilers.
              | ident.Nat_succ
              | ident.Nat_add
              | ident.Nat_mul
+             | ident.Nat_max
              | ident.bool_rect _
              | ident.nat_rect _
              | ident.pred
@@ -5219,7 +5267,15 @@ Module Compilers.
                        let result := ident.interp idc (x, y, z, a) in
                        inr (inr (fst result), inr (snd result))
                      | inr (inr (inr (inr x, y), z), a)
-                        => default_interp (ident.Z.add_with_get_carry_concrete x) (inr (inr (y, z), a))
+                       => let default := default_interp (ident.Z.add_with_get_carry_concrete x) (inr (inr (y, z), a)) in
+                          match (z, a) with
+                          | (inr xx, inl e)
+                          | (inl e, inr xx)
+                            => if Z.eqb xx 0
+                               then inr (inl e, inr 0%Z)
+                               else default
+                          | _ => default
+                          end
                      | _ => default_interp idc x_y_z_a
                      end
              | ident.Z_sub_get_borrow as idc
@@ -5300,9 +5356,10 @@ Module Compilers.
                      end
              | ident.Nat_add as idc
              | ident.Nat_mul as idc
+             | ident.Nat_max as idc
+             | ident.Z_pow as idc
              | ident.Z_eqb as idc
              | ident.Z_leb as idc
-             | ident.Z_pow as idc
                => fun (x_y : data (_ * _) * expr (_ * _) + (_ + type.interp _) * (_ + type.interp _))
                   => match x_y return _ + type.interp _ with
                      | inr (inr x, inr y) => inr (ident.interp idc (x, y))
@@ -8079,18 +8136,19 @@ Module Montgomery256.
   Set Printing Width 100000.
 
   Print montred256.
-  (*montred256 = fun var : type -> Type => λ x : var (type.type_primitive type.Z * type.type_primitive type.Z)%ctype,
+  (*
+montred256 = fun var : type -> Type => λ x : var (type.type_primitive type.Z * type.type_primitive type.Z)%ctype,
              expr_let x0 := (uint128)(x₁ >> 128) in
              expr_let x1 := ((uint128)(x₁) & 340282366920938463463374607431768211455) in
              expr_let x2 := 79228162514264337593543950337 *₂₅₆ x0 in
              expr_let x3 := ((uint128)(x2) & 340282366920938463463374607431768211455) in
              expr_let x4 := 340282366841710300986003757985643364352 *₂₅₆ x1 in
              expr_let x5 := ((uint128)(x4) & 340282366920938463463374607431768211455) in
-             expr_let x6 := (uint256)(x5 << 128) in
-             expr_let x7 := (uint256)(x3 << 128) in
-             expr_let x8 := 79228162514264337593543950337 *₂₅₆ x1 in
-             expr_let x9 := ADD_256 (x6, x7) in
-             expr_let x10 := ADD_256 (x8, x9₁) in
+             expr_let x6 := (uint256)(x3 << 128) in
+             expr_let x7 := 79228162514264337593543950337 *₂₅₆ x1 in
+             expr_let x8 := ADDC_256 (0, x6, x7) in
+             expr_let x9 := (uint256)(x5 << 128) in
+             expr_let x10 := ADDC_256 (0, x9, x8₁) in
              expr_let x11 := (uint128)(x10₁ >> 128) in
              expr_let x12 := ((uint128)(x10₁) & 340282366920938463463374607431768211455) in
              expr_let x13 := 79228162514264337593543950335 *₂₅₆ x11 in
@@ -8099,23 +8157,21 @@ Module Montgomery256.
              expr_let x16 := 340282366841710300967557013911933812736 *₂₅₆ x12 in
              expr_let x17 := (uint128)(x16 >> 128) in
              expr_let x18 := ((uint128)(x16) & 340282366920938463463374607431768211455) in
-             expr_let x19 := (uint256)(x18 << 128) in
-             expr_let x20 := (uint256)(x15 << 128) in
-             expr_let x21 := 79228162514264337593543950335 *₂₅₆ x12 in
-             expr_let x22 := ADD_256 (x19, x20) in
-             expr_let x23 := ADD_256 (x21, x22₁) in
-             expr_let x24 := x23₂ +₁₂₈ x22₂ in
-             expr_let x25 := 340282366841710300967557013911933812736 *₂₅₆ x11 in
-             expr_let x26 := ADD_256 (x14, x25) in
-             expr_let x27 := ADD_256 (x17, x26₁) in
-             expr_let x28 := ADD_256 (x24, x27₁) in
-             expr_let x29 := ADD_256 (x₁, x23₁) in
-             expr_let x30 := ADDC_256 (x29₂, x₂, x28₁) in
-             expr_let x31 := SELC (x30₂, 0, 115792089210356248762697446949407573530086143415290314195533631308867097853951) in
-             expr_let x32 := Z.cast uint256 @@ (fst @@ SUB_256 (x30₁, x31)) in
-             ADDM (x32, 0, 115792089210356248762697446949407573530086143415290314195533631308867097853951)
+             expr_let x19 := (uint256)(x15 << 128) in
+             expr_let x20 := 79228162514264337593543950335 *₂₅₆ x12 in
+             expr_let x21 := ADDC_256 (0, x19, x20) in
+             expr_let x22 := 340282366841710300967557013911933812736 *₂₅₆ x11 in
+             expr_let x23 := ADDC_256 (x21₂, x22, x17) in
+             expr_let x24 := (uint256)(x18 << 128) in
+             expr_let x25 := ADDC_256 (0, x24, x21₁) in
+             expr_let x26 := ADDC_256 (x25₂, x14, x23₁) in
+             expr_let x27 := ADD_256 (x₁, x25₁) in
+             expr_let x28 := ADDC_256 (x27₂, x₂, x26₁) in
+             expr_let x29 := SELC (x28₂, 0, 115792089210356248762697446949407573530086143415290314195533631308867097853951) in
+             expr_let x30 := Z.cast uint256 @@ (fst @@ SUB_256 (x28₁, x29)) in
+             ADDM (x30, 0, 115792089210356248762697446949407573530086143415290314195533631308867097853951)
      : Expr (type.type_primitive type.Z * type.type_primitive type.Z -> type.type_primitive type.Z)
-*)
+   *)
 End Montgomery256.
 
 (* Extra-specialized ad-hoc pretty-printing *)
@@ -8219,17 +8275,18 @@ Local Open Scope expr_scope.
 
 Print Montgomery256.montred256.
 (*
+<<<<<<< HEAD
 c.ShiftR($x0, $x_lo, 128);
 c.Lower128($x1, $x_lo);
 c.Mul128x128($x2, Lower128{RegPinv}, $x0);
 c.Lower128($x3, $x2);
 c.Mul128x128($x4, RegPinv >> 128, $x1);
 c.Lower128($x5, $x4);
-c.ShiftL($x6, $x5, 128);
-c.ShiftL($x7, $x3, 128);
-c.Mul128x128($x8, Lower128{RegPinv}, $x1);
-c.Add256($x9, $x6, $x7);
-c.Add256($x10, $x8, $x9_lo);
+c.ShiftL($x6, $x3, 128);
+c.Mul128x128($x7, Lower128{RegPinv}, $x1);
+c.Addc($x8, $x6, $x7);
+c.ShiftL($x9, $x5, 128);
+c.Addc($x10, $x9, $x8_lo);
 c.ShiftR($x11, $x10_lo, 128);
 c.Lower128($x12, $x10_lo);
 c.Mul128x128($x13, Lower128{RegMod}, $x11);
@@ -8238,22 +8295,18 @@ c.Lower128($x15, $x13);
 c.Mul128x128($x16, RegMod << 128, $x12);
 c.ShiftR($x17, $x16, 128);
 c.Lower128($x18, $x16);
-c.ShiftL($x19, $x18, 128);
-c.ShiftL($x20, $x15, 128);
-c.Mul128x128($x21, Lower128{RegMod}, $x12);
-c.Add256($x22, $x19, $x20);
-c.Add256($x23, $x21, $x22_lo);
-c.Add64($x24, $x23_hi, $x22_hi);
-c.Mul128x128($x25, RegMod << 128, $x11);
-c.Add256($x26, $x14, $x25);
-c.Add256($x27, $x17, $x26_lo);
-c.Add256($x28, $x24, $x27_lo);
-c.Add256($x29, $x_lo, $x23_lo);
-c.Addc($x30, $x_hi, $x28_lo);
-c.Selc($x31,RegZero, RegMod);
-c.Sub($x32, $x30_lo, $x31);
-c.AddM($ret, $x32, RegZero, RegMod);
-     : Expr
-         (type.type_primitive type.Z * type.type_primitive type.Z ->
-          type.type_primitive type.Z)
+c.ShiftL($x19, $x15, 128);
+c.Mul128x128($x20, Lower128{RegMod}, $x12);
+c.Addc($x21, $x19, $x20);
+c.Mul128x128($x22, RegMod << 128, $x11);
+c.Addc($x23, $x22, $x17);
+c.ShiftL($x24, $x18, 128);
+c.Addc($x25, $x24, $x21_lo);
+c.Addc($x26, $x14, $x23_lo);
+c.Add256($x27, $x_lo, $x25_lo);
+c.Addc($x28, $x_hi, $x26_lo);
+c.Selc($x29,RegZero, RegMod);
+c.Sub($x30, $x28_lo, $x29);
+c.AddM($ret, $x30, RegZero, RegMod);
+     : Expr (type.type_primitive type.Z * type.type_primitive type.Z -> type.type_primitive type.Z)
  *)
